Added push and pop methods for queues Push method defined Push method preserves WF_queue TODO: Pop

opaque.dfy
@@ -8,40 +8,61 @@
 abstract module Opaque{
     ////CONFIG////
     type Config
-    function Heap(i: Addr, fid: FId) : Addr 
+    type Actor 
+    type Frame
+    datatype Msg = orca(i: Addr, z: int) | app(f: Frame) | ERR 
+    type FId 
+    function Heap(c: Config, i: Addr, fid: FId) : Addr 
     
 
     ////ADDRESSES////
     datatype Addr = OA(ObjectAddr) | AA(ActorAddr) | Null
-    type ObjectAddr
+    type ObjectAddr 
     type ActorAddr
     
 
     ////ACTORS////
-    datatype Actor = Actor(q: Queue, st: State)
+//    datatype Actor = Actor(st: State, cl: ClassId)
     //lemma RANGE OF ACTORS IS FINITE
     //lemma all valid actor addresses are in the domain of Actors
-    function Actors(a: ActorAddr, c: Config) : Actor
+    function Actors(c: Config, a: ActorAddr) : Actor
 
     //Queues//
     //length added to convince Dafny that queues are finite 
     //Is there a better way?
-    datatype Queue = Queue(msg: Msg, length: int) //opaque - how?
-    //??
-    predicate WF_queue(c: Config, a: ActorAddr) {
-        exists n:nat :: NthMsg(c, a, n) != Msg.ERR && n >= 1 ==> NthMsg(c, a, n-1) != Msg.ERR 
-                                                                && n <= queue_length(c, a)
-    }
-
+    //datatype Queue = Queue(msg: Msg, length: int) //opaque - how?
+    function queue_length(c: Config, a: ActorAddr) : nat 
+    function queue_n(c: Config, a: ActorAddr, n: nat) : Msg 
 
     function prev_message(c: Config, a: ActorAddr, n: nat) : Msg
     {
-        if n >= 1 then NthMsg(c, a, n-1) else Msg.ERR
+        if n >= 1 then queue_n(c, a, n-1) else Msg.ERR
     }
 
-    predicate WF_queue'(c: Config, a: ActorAddr) {
-        forall n:nat :: NthMsg(c, a, n) == Msg.ERR ==> NthMsg(c,a,n+1) == Msg.ERR
+    predicate WF_queue(c: Config, a: ActorAddr) {
+        (forall n:nat :: n < queue_length(c,a) ==> queue_n(c, a, n) != Msg.ERR) &&
+        (forall n:nat :: n >= queue_length(c,a) ==> queue_n(c,a,n) == Msg.ERR)
     }
+
+    predicate push(c: Config, a: ActorAddr, msg: Msg, c': Config)
+    {
+        WF_queue(c,a) && msg != Msg.ERR &&
+        queue_length(c', a) == queue_length(c, a) + 1 && queue_n(c', a, queue_length(c,a)) == msg &&
+        forall n:nat :: n != queue_length(c,a) ==> queue_n(c',a,n) == queue_n(c,a,n) 
+    }
+
+    lemma push_preserves_WF_queue(c: Config, a: ActorAddr, msg: Msg, c': Config) 
+        requires push(c, a, msg, c')
+        ensures WF_queue(c', a)
+    {
+    }
+    
+//TODO: Complete pop
+    predicate pop(c:Config, a:ActorAddr, msg: Msg, c': Config){true} 
+        
+
+
+    /*
 
 
     //States// 
@@ -71,6 +92,7 @@ abstract module Opaque{
     datatype DP = This | LP(zero: int, x: VarId) | MP(k: int, x': VarId) | cons(dp: DP, f: FId)
     datatype SP = This | bsp(b: BId, x: VarId) | cons(sp: SP, f: FId)
     datatype Capability = WRITE | READ | TAG | ERR
+    
 
 
     ////REFERENCE COUNTS////
@@ -84,16 +106,48 @@ abstract module Opaque{
     function Owner(c: Config, i: Addr) : ActorAddr
     function Field(c: Config, i: Addr, f: FId) : Addr //what do we need this for?
     function Class(c: Config, a: ActorAddr) : ClassId 
-    function NthMsg(c: Config, a: ActorAddr, n: nat) : Msg 
     function Addrs(c: Config) : set<ActorAddr>
     
     predicate Reach(c: Config, a: ActorAddr, n: nat, i: Addr)
 
+    ////DATA-RACE FREEDOM//// 
+    function sees(cid: ClassId, sp: SP) : Capability
+    function views(c: Config, a: ActorAddr, p:DP) : Capability
     
+    lemma {:verify true} A1(a: Actor, sp: SP, f: FId, cappa: Capability) 
+    requires sees(a.cl, SP.cons(sp, f)) == cappa //pass cappa as param instead?
+    ensures exists cappa' :: cappa' != TAG && sees(a.cl, sp) == cappa' 
+
+
+    lemma {:verify true} A2(a: Actor, sp: SP, f: FId) 
+    requires sees(a.cl, SP.cons(sp, f)) == WRITE
+    ensures sees(a.cl, sp) == WRITE
+
+    function C(c: Config, a: ActorAddr, dp: DP) : Addr 
+    function A(c: Config, a: ActorAddr, dp: DP) : (Addr, Capability)
+   /*
+     predicate WF_A(c: Config, a: ActorAddr, dp: DP) {
+        forall i: Addr :: ((exists k: Capability :: 
+        A(c,a,dp) == (i, k)) <==> (C(c,a,dp) == i && views(c,a,dp) == k 
+                                || k == TAG && exists k', i', p' ::
+                                (p == Cons(p',) && A(c,a,p') == (i', k') && Owner(c, i') == i)))
+                                                                      
+    }
+    */
+    /*
+    predicate DFR(c: Config) {
+        forall a, a': ActorAddr, p, p': DP, i: Addr :: (a != a' && (exists k :: A(c, a, p) == (i, k) && k==WRITE) 
+                                            ==> (exists k' :: A(c, a', p') == (i, k') ==> k' == TAG))
+    } */
+    predicate DFR(c: Config) {
+        forall a, a': ActorAddr, p, p': DP, i: Addr :: (a != a' && (exists k :: A(c, a, p) == (i, k) && k==WRITE) 
+                                            && exists k' :: A(c, a', p') == (i, k') ==> k' == TAG)
+    }
+
     ////AUXILIARY FUNCTION////
     //TODO: separate into its own module
     function queue_length(c: Config, a: ActorAddr) : int {
         Actors(a,c).q.length
     }
-    
-}
+  */  
+} 
